src/syntax/syntax.fs
@@ -107,8 +107,9 @@ and comp_typ = {
   flags:list<cflags>
 }
 and comp' =
-  | Total of typ
-  | Comp of comp_typ
+  | Total  of typ
+  | GTotal of typ
+  | Comp   of comp_typ
 and term = syntax<term',term'>
 and typ = term                                                   (* sometimes we use typ to emphasize that a term is a type *)
 and pat = withinfo_t<pat',term'>
@@ -359,7 +360,8 @@ let extend_app t arg kopt r = match t.n with
     | Tm_app(head, args) -> mk_Tm_app head (args@[arg]) kopt r
     | _ -> mk_Tm_app t [arg] kopt r
 let mk_Tm_delayed lr pos : term = mk (Tm_delayed(lr, Util.mk_ref None)) None pos
-let mk_Total t : comp = mk (Total t) None t.pos
+let mk_Total t : comp  = mk (Total t) None t.pos
+let mk_GTotal t : comp = mk (GTotal t) None t.pos
 let mk_Comp (ct:comp_typ) : comp  = mk (Comp ct) None ct.result_typ.pos
 let mk_lb (x, univs, eff, t, e) = {lbname=x; lbunivs=univs; lbeff=eff; lbtyp=t; lbdef=e}
 let mk_subst (s:subst)   = s
