src/typechecker/util.fs
@@ -528,9 +528,15 @@ let bind env e1opt (lc1:lcomp) ((b, lc2):lcomp_with_binder) : lcomp =
             else if Util.is_ml_comp c1 && Util.is_ml_comp c2
             then Some c2
             else None in
-        match e1opt, b with
+        if Util.is_total_comp c1
+        && Util.is_total_comp c2
+        then Some c2
+        else if Util.is_tot_or_gtot_comp c1
+             && Util.is_tot_or_gtot_comp c2
+        then Some (S.mk_GTotal (Util.comp_result c2))
+        else match e1opt, b with
             | Some e, Some x ->
-                if Util.is_tot_or_gtot_comp c1 && not (Syntax.is_null_bv x)
+                if Util.is_total_comp c1 && not (Syntax.is_null_bv x)
                 then Some <| SS.subst_comp [NT(x, e)] c2
                 else aux ()
             | _ -> aux () in
@@ -576,7 +582,8 @@ let refresh_comp_label env (b:bool) lc =
         let c = lc.comp () in
         if Util.is_ml_comp c then c
         else match c.n with
-        | Total _ -> c
+        | Total _ 
+        | GTotal _ -> c
         | Comp ct ->
           if Env.debug env Options.Low
           then (Util.print1 "Refreshing label at %s\n" (Range.string_of_range <| Env.get_range env));
@@ -756,6 +763,8 @@ let maybe_assume_result_eq_pure_term env (e:term) (lc:lcomp) : lcomp =
       if not (is_pure_or_ghost_effect env lc.eff_name)
       then c
       else if Util.is_partial_return c then c
+      else if Util.is_tot_or_gtot_comp c && Option.isNone <| Env.lookup_effect_abbrev env Const.effect_GTot_lid
+      then failwith (Printf.sprintf "%s: %s\n" (Range.string_of_range e.pos) (Print.term_to_string e))
       else
            let c = Normalize.unfold_effect_abbrev env c in
            let t = c.result_typ in
@@ -858,6 +867,7 @@ let pure_or_ghost_pre_and_post env comp =
     if Util.is_tot_or_gtot_comp comp
     then None, Util.comp_result comp
     else begin match comp.n with
+            | GTotal _
             | Total _ -> failwith "Impossible"
             | Comp ct ->
               if lid_equals ct.effect_name Const.effect_Pure_lid
