lib/FStar.All.fst
@@ -21,21 +21,21 @@ module FStar.All
 open FStar.Heap
 open FStar.ST
 
-kind AllPre = AllPre_h heap
-kind AllPost (a:Type) = AllPost_h heap a
-kind AllWP (a:Type) = AllWP_h heap a
+let all_pre = all_pre_h heap
+let all_post (a:Type) = all_post_h heap a
+let all_wp (a:Type) = all_wp_h heap a
 new_effect ALL = ALL_h heap
 
-let lift_state_all (a:Type) (wp:STWP a) (p:AllPost a) =  wp (fun a -> p (V a))
+let lift_state_all (a:Type) (wp:st_wp a) (p:all_post a) =  wp (fun a -> p (V a))
 sub_effect STATE ~> ALL = lift_state_all
 
-let lift_exn_all (a:Type) (wp:ExWP a)   (p:AllPost a) (h:heap) = wp (fun ra -> p ra h)
+let lift_exn_all (a:Type) (wp:ex_wp a)   (p:all_post a) (h:heap) = wp (fun ra -> p ra h)
 sub_effect EXN   ~> ALL = lift_exn_all
 
-effect All (a:Type) (pre:AllPre) (post: (heap -> Tot (AllPost a))) =
+effect All (a:Type) (pre:all_pre) (post: (heap -> Tot (all_post a))) =
        ALL a
-           (fun (p:AllPost a) (h:heap) -> pre h /\ (forall ra h1. post h ra h1 ==> p ra h1)) (* AllWP *)
-           (fun (p:AllPost a) (h:heap) -> forall ra h1. (pre h /\ post h ra h1) ==> p ra h1) (* WLP *)
+           (fun (p:all_post a) (h:heap) -> pre h /\ (forall ra h1. post h ra h1 ==> p ra h1)) (* WP  *)
+           (fun (p:all_post a) (h:heap) -> forall ra h1. (pre h /\ post h ra h1) ==> p ra h1) (* WLP *)
 default effect ML (a:Type) =
   ALL a (all_null_wp heap a) (all_null_wp heap a)
 
