lib/FStar.Squash.fst
@@ -1,29 +1,47 @@
-(*--build-config
-    options:--warn_top_level_effects;
-    other-files:FStar.Squash.fsti;
---*)
+(* Interface for squash types; somehow inspired by:
+   Quotient Types: A Modular Approach. Aleksey Nogin, TPHOLs 2002.
+   http://www.nuprl.org/documents/Nogin/QuotientTypes_02.pdf
+*)
 module FStar.Squash
 
 (* This file shows that there is a natural model for some of the squash things;
-   DO NOT IMPORT THIS FILE; USE FStar.Squash.fsti and --admit_fsi FStar.Squash INSTEAD
  *)
 
-type squash (t:Type) = t
+abstract type squash (t:Type) = t
 
-let return_squash x = x
+abstract val give_proof : #p:Type -> squash p ->
+  Pure unit (requires True) (ensures (fun _ -> p))
 
-let bind_squash x f = f x
+abstract val proof_irrelevance : p:Type -> x:squash p ->
+                                 y:squash p -> Tot (squash (x = y))
 
-let map_squash x f = f x
+abstract val squash_double_arrow : #a:Type -> #p:(a -> Type) ->
+  =f:(squash (x:a -> Tot (squash (p x)))) -> Tot (squash (x:a -> Tot (p x)))
 
-(* Inconsistent, see #355 *)
-assume val get_proof : p:Type ->
-  Pure (squash p) (requires p) (ensures (fun _ -> True))
+(* This is a monad, but not an effect *)
 
-let give_proof (#p:Type) (s:squash p) = ()
+abstract val return_squash : #a:Type -> a -> Tot (squash a)
+
+abstract val bind_squash : #a:Type -> #b:Type -> squash a -> (a -> Tot (squash b)) ->
+  Tot (squash b)
+
+abstract val map_squash : #a:Type -> #b:Type -> squash a -> (a -> Tot b) ->
+  Tot (squash b)
+
+let return_squash #a x = x
+
+let bind_squash #a #b x f = f x
+
+let map_squash #a #b x f = f x
+
+let give_proof #p s = ()
+
+let squash_double_arrow #a #p f = f
 
 (* Inconsistent *)
 assume val proof_irrelevance : p:Type -> x:squash p ->
                                         y:squash p -> Tot (squash (x = y))
 
-let squash_double_arrow (#a:Type) (#p:a -> Type) f = f
+(* Inconsistent, see #355 *)
+assume val get_proof : p:Type ->
+  Pure (squash p) (requires p) (ensures (fun _ -> True))
