lib/FStar.Int8.fst
@@ -30,7 +30,7 @@ type nat8 = x:int8{Prims.op_GreaterThanOrEqual (as_int x) 0}
 
 //a ?+ b may overflow
 //must be marked opaque because the body has an intentional admit
-opaque val op_Question_Plus: i:int8
+abstract val op_Question_Plus: i:int8
               -> j:int8
               -> Tot (k:int8{within_int8 (as_int i + as_int j) ==> as_int k = as_int i + as_int j})
 let op_Question_Plus (Int8 i) (Int8 j) =
@@ -45,7 +45,7 @@ let op_Plus (Int8 i) (Int8 j) = Int8 (i + j)
 
 //a ?- b may overflow
 //must be marked opaque because the body has an intentional admit
-opaque val op_Question_Subtraction: i:int8
+abstract val op_Question_Subtraction: i:int8
               -> j:int8
               -> Tot (k:int8{within_int8 (as_int i - as_int j) ==> as_int k = as_int i - as_int j})
 let op_Question_Subtraction (Int8 i) (Int8 j) =
@@ -60,7 +60,7 @@ let op_Subtraction (Int8 i) (Int8 j) = Int8 (i - j)
 
 //a ?* b may overflow
 //must be marked opaque because the body has an intentional admit
-opaque val op_Question_Star:
+abstract val op_Question_Star:
                  i:int8
               -> j:int8
               -> Tot (k:int8{within_int8 (as_int i * as_int j) ==> as_int k = as_int i * as_int j})
@@ -76,7 +76,7 @@ let op_Star (Int8 i) (Int8 j) = Int8 (i * j)
 
 //When the dividend is negative, the semantics is platform dependent
 //must be marked opaque because the body has an intentional admit
-opaque val op_Question_Slash: i:int8
+abstract val op_Question_Slash: i:int8
                            -> j:int8{as_int j <> 0}
                            -> Tot (k:int8{as_int i >= 0 ==> as_int k = as_int i / as_int j})
 let op_Question_Slash (Int8 i) (Int8 j) =
@@ -92,7 +92,7 @@ let op_Slash (Int8 i) (Int8 j) = Int8 (i / j)
 
 //a ?% b can overflow
 //must be marked opaque because the body has an intentional admit
-opaque val op_Question_Percent:
+abstract val op_Question_Percent:
                 i:int8
              -> j:int8{as_int j <> 0}
              -> Tot (k:int8{not(as_int i = min_value_int && as_int j = -1)
@@ -113,7 +113,7 @@ let op_Percent (Int8 i) (Int8 j) = Int8 (i % j)
 
 //?- a    can overflow
 //must be marked opaque because the body has an intentional admit
-opaque val op_Question_Minus: i:int8
+abstract val op_Question_Minus: i:int8
                    -> Tot int8
 let op_Question_Minus (Int8 i) =
   if i = min_value_int
